$$
\lim_{x \to c} x = c
$$

Proof:
$$
\forall \epsilon > 0, \exists \delta > 0, s.t. 0 < | x - c| < d \rightarrow |x-c| < \epsilon
$$
choose $d$ to be $x -c$
$$
|x - c| < \epsilon
$$
$$
d = \epsilon
$$

QED


$$
\lim_{x \to c} k = k
$$
k is a constant

Proof:
$$
\forall \epsilon > 0, \exists \delta > 0, s.t. 0 < | x - c| < d \rightarrow |k-k| < \epsilon
$$

$$
\lim_{x \to c} mx + b = mc + b
$$

$$
\forall \epsilon > 0, \exists \delta > 0, s.t. 0 < | x - c| < d \rightarrow |mx+b - (mc+b)| < \epsilon |mx + b - (mc+b)|
$$
$$
|mx+b - (mc+b)|
$$
$$
= |mx+b - mc-b|
$$
$$
=|mx - mc|
$$
$$
= |m(x-c)
$$
$$
= m|x-c|
$$
$$
=md
$$
$$
md = \epsilon
$$
$$
d = \frac{\epsilon}{m}
$$

$$
|mx+b - (mc+b)| < \epsilon
$$

$$
|m(x-c)|<\epsilon
$$
$$
m \left(\frac{\epsilon}{m}\right)= \epsilon
$$

QED
